

---
Monotone Convergence Theorem for Sequences of Measurable Sets
---

Given $\left(X, \mathfrak{A}, \mu\right)$ be a measure space.
Let $\{E_n: n \in \mathbb{N}\}$ be a sequence in $\mathfrak{A}.$



`1.`

If $\{E_n\}$ is monotonically increasing, then
$$
\lim_{n\rightarrow \infty} \mu \left(E_n\right)
= \mu \left(\lim_{n\rightarrow \infty} E_n\right).
$$

`2`.

If $\{E_n\}$ is monotonically decreasing, and there exists a set $A \in \mathfrak{A}$ with $\mu\left(A\right)<\infty$ such that $E_1\subset A,$ then

$$
\lim_{n\rightarrow \infty} \mu \left(E_n\right)
= \mu \left(\lim_{n\rightarrow \infty} E_n\right).
$$



\
\
\
\
\
\
\
\
\
\
\
\




---
Proof
---

`1.`

First, consider there exists $n_0\in \mathbb{N}$ such that

$$
\mu\left(E_{n_0}\right)=\infty
$$

then

$$
\lim_{n\rightarrow \infty}
\mu\left(E_n\right)=\infty.
$$

On the other hand,

$$
\begin{aligned}
\infty
&= \mu\left(E_{n_0}\right) \\
&\leq
\mu\left( 
    \bigcup_{n \in \mathbb{N}} E_n
\right) \\
&=
\mu \left(\lim_{n\rightarrow \infty} E_n\right).
\end{aligned}
$$

Thus

$$
\lim_{n\rightarrow \infty} \mu \left(E_n\right)
= \mu \left(\lim_{n\rightarrow \infty} E_n\right).
$$


Second, consider for all $n\in\mathbb{N}$

$$
\mu\left(
    E_n
\right)
< \infty.
$$

Define for all $n \in \mathbb{N}$

<!-- $$
\{ \ 
    F_n: n \in \mathbb{N}
\ \}
$$

such that -->

$$
F_n
:= E_n \backslash E_{n-1}
$$

with

$$
E_0 := \emptyset
$$

then

$$
\bigcup_{n\in \mathbb{N}}
E_n
= \bigsqcup_{n\in \mathbb{N}}
F_n.
$$

Therefore,

$$
\begin{aligned}
\mu\left(
    \lim_{n \rightarrow \infty} E_n
\right)
&= \mu\left(
    \bigcup_{n \in \mathbb{N}}
    E_n
\right) \\
&= \mu\left(
    \bigsqcup_{n \in \mathbb{N}}
    F_n
\right) \\
&= \sum_{n \in \mathbb{N}}
\mu\left(
    F_n
\right) \\
&= \sum_{n \in \mathbb{N}}
\mu\left(
    E_n \backslash E_{n-1} 
\right) \\
&= \sum_{n \in \mathbb{N}}
\mu\left(E_n\right)
-\mu\left(E_{n-1}\right) \\
&= \lim_{n \rightarrow \infty}
\sum_{k=1}^n
\mu\left(E_k\right)
-\mu\left(E_{k-1}\right) \\
&= \lim_{n\rightarrow \infty}
\left(\mu\left(E_n\right)
-\mu\left(E_0\right)\right) \\
&= \lim_{n\rightarrow \infty}
\mu\left(E_n\right).
\end{aligned}
$$

Thus we proved.

`2.`

We define for all $n \in \mathbb{N}$

$$
F_n
:= E_n \backslash E_{n+1}
$$

then

$$
\bigcap_{n \in \mathbb{N}}
E_n
= E_1
\backslash
\left(
    \bigsqcup_{n \in \mathbb{N}}
    F_n
\right).
$$

Therefore

$$
\begin{aligned}
\mu\left(
    \lim_{n \rightarrow \infty}
    E_n
\right)
&= \mu\left(
    \bigcap_{n \in \mathbb{N}}
    E_n
\right) \\
&= \mu\left(
    E_1
    \backslash
    \left(
        \bigsqcup_{n \in \mathbb{N}}
        F_n
    \right)
\right)\\
&= \mu\left(
    E_1
\right)
-\mu\left(
    \bigsqcup_{n \in \mathbb{N}}
    F_n
\right) \\
&= \mu\left(
    E_1
\right)
-\sum_{n \in \mathbb{N}}
\mu\left(F_n\right) \\
&= \mu\left(
    E_1
\right)
-\sum_{n \in \mathbb{N}}
\mu\left(E_n\backslash E_{n-1}\right)\\
&= \mu\left(
    E_1
\right)
-\sum_{n \in \mathbb{N}}
\mu\left(E_n\right)
-\mu\left(E_{n-1}\right) \\
&= \mu\left(
    E_1
\right)
-\lim_{n \rightarrow \infty}
\sum_{k =1}^{n}
\mu\left(E_k\right)
-\mu\left(E_{k-1}\right) \\
&= \mu\left(
    E_1
\right)
-\lim_{n \rightarrow \infty}\left(
    \mu\left(E_1\right)
    -\mu\left(E_n\right)
\right)\\
&= \mu\left(
    E_1
\right)
-\left(
    \mu\left(E_1\right)
    -\lim_{n \rightarrow \infty}
    \mu\left(E_n\right)
\right) \\
&= \lim_{n \rightarrow \infty}
    \mu\left(E_n\right).
\end{aligned}
$$

Thus we proved.

</span>