
---
Translation Invariance of the Lebesgue Measure
---

Given $\left(\mathbb{R}, \mathfrak{M}_L, \mu_L\right)$ be the Lebesgue measure space. Let $E + x:= \{ \ 
    e + x : e \in E
\ \}$ and $
\mathfrak{M}_L + x
:= \{ \ 
    E + x : E\in \mathfrak{M}_L    
\ \}
$ for $E \in \mathfrak{M}_L$ and $x \in \mathbb{R}$.

Then

`1.`

$$
E + x \in \mathfrak{M}_L
$$

and

$$
\mu_L\left(E+x\right)
= \mu_L\left(E\right).
$$

<!-- for $E \in \mathfrak{M}_L$, $x\in\mathbb{R}$. -->


`2.`

$$
\mathfrak{M}_L + x
= \mathfrak{M}_L.
$$


---
Proof
---

`1.`

Let $\mu^*_L$ be the Lebesgue outer measure.

For any $A\in\mathcal{\mathcal{P}}\left(\mathbb{R}\right)$

$$
\begin{aligned}
\mu^*_L&\left(A \cap \left(E+x\right)\right)
+
\mu^*_L\left(A \cap \left(E+x\right)^c\right) \\
&=
\mu^*_L\left(A \cap \left(E+x\right)\right)
+
\mu^*_L\left(A \cap \left(E^c + x\right)\right) \\
&=
\mu^*_L\left(\left(A \cap \left(E+x\right)\right)-x\right)
+
\mu^*_L\left(\left(A \cap \left(E^c + x\right)\right)-x\right) \\
&=
\mu^*_L\left(\left(A - x\right)\cap E\right)
+
\mu^*_L\left(\left(A - x\right) \cap E^c\right) \\
&=
\mu^*_L\left(A - x\right) \\
&=
\mu^*_L\left(A\right)
\end{aligned}
$$

then

$$
E + x \in \mathfrak{M}_L
$$

also

$$
\begin{aligned}
\mu_L\left(E+x\right)
&=
\mu^*_L\left(E+x\right) \\
&=
\mu^*_L\left(E\right) \\
&=
\mu_L\left(E\right).
\end{aligned}
$$

Thus we proved.

`2.`

It can be proved in the same way of `1.`.

