
---
Approximation By Right-Continuous Step Function
---

Let $f$ be an extended real-valued $\mathfrak{M}_L$-measurable function on $D:=[a, b)$ for some $a, b\in\mathbb{R}$, and $f$ takes values in $\mathbb{R}$ a.e.

Then

`1.`

For arbitrary $\epsilon>0$ there exists a right-continuous step function $g$ on $D$ and $E\in\mathfrak{M}_L$ with $\mu(E)<\epsilon$ such that

$$\begin{aligned}
\left| f - g\right| <\epsilon \ \ on \ D\backslash E.
\end{aligned}$$

`2.`

Moreover, if $M_1\leq f \leq M_2 \ on \ D$ for some $M_1, M_2 \in \mathbb{R}$, $g$ can be chosen as

$$\begin{aligned}
M_1 \leq g \leq M_2 \ \ on \ D
\end{aligned}$$

<br>
<br>
<br>
<br>
<br>
<br>
<br>
<br>
<br>
<br>
<br>
<br>
<br>
<br>
<br>
<br>


---
Proof
---

`1.`

First, consider the case $f$ is non-negative.

For $\epsilon>0$, let $M\in\mathbb{R}$ such that there exists $E\in\mathfrak{M}_L$ with $\mu_L(E)<\epsilon$ and

$$\begin{aligned}
0 \leq f < M \ \ on \ D\backslash E.
\end{aligned}$$

Let $N\in\mathbb{N}$ be so large that $M/N<\epsilon$, and

$$\begin{aligned}
D_n
&:= f^{-1}\left(
    \left[
        n\frac{M}{N}, (n+1)\frac{M}{N}
    \right)
\right)
\ \ {\rm for} \ n\in\{0,1,\cdots,N-1\} \\
D_N
&:= E \\
D^b &:= \bigsqcup_{n=1}^{N-1}D_n
\end{aligned}$$

then

$$\begin{aligned}
\mu_L(D^b) > \mu_L(D) - \epsilon.
\end{aligned}$$

Notice that

$$\begin{aligned}
\bigsqcup_{n=0}^{N} D_n
= D.
\end{aligned}$$

For arbitrary $\epsilon'>0$, let $V_n$ be a union of finitely many left-closed right-opened intervals such that

$$\begin{aligned}
\mu_L(D_n\triangle V_n) < \epsilon'.
\end{aligned}$$

Define $\mathfrak{M}_L$-measurable function $s_n$ on $D$ as

$$\begin{aligned}
s_n(x)
:= \left\{
\begin{array}{l}
n\frac{M}{N} \ \ {\rm for} \ x\in D \cap V_n. \\
0 \ \ \ \ \ \ {\rm else}
\end{array}
\right.
\end{aligned}$$

also right-continuous function $s$ on $D$ as

$$\begin{aligned}
s(x)
:= \sum_{n=1}^{N} s_n(x).
\end{aligned}$$

Define mutually disjoint $\mathfrak{M}_L$-measurable set $D^*_n$ as 

$$\begin{aligned}
D^*_n
&:= \left\{
    D_n \cap V_n
\right\} \backslash \bigcup_{k\neq n} V_k \\
&= \left\{
    D_n \cap V_n
\right\} \backslash \bigcup_{k\neq n} \left\{
    V_k \cap D_k \cup V_k \backslash D_k
\right\} \\
&= \left\{
    D_n \cap V_n
\right\} \backslash \bigcup_{k\neq n} \left\{
    V_k \backslash D_k
\right\}
\end{aligned}$$

Therefore

$$\begin{aligned}
\mu_L(D^*_n)
&= \mu_L\left(
    \left\{
        D_n \cap V_n
    \right\} \backslash \bigcup_{k\neq n} \left\{
        V_k \backslash D_k
    \right\}
\right) \\
&= \mu_L\left(
    D_n \cap V_n
\right) - \mu\left(
    \bigcup_{k\neq n} \left\{
        V_k \backslash D_k
    \right\}
\right) \\
&\geq \mu_L\left(
    D_n \backslash \left\{
        V_n \triangle D_n
    \right\}
\right) - \sum_{k\neq n}\mu\left(
    V_k \backslash D_k
\right) \\
&\geq \mu_L\left(
    D_n
\right) - \mu_L(V_n \triangle D_n) - \sum_{k\neq n}\mu\left(
    V_k \triangle D_k
\right) \\
&= \mu_L\left(
    D_n
\right) - \sum_{k=0}^N\mu\left(
    V_k \triangle D_k
\right) \\
&= \mu_L\left(
    D_n
\right) - (N+1)\epsilon'
\end{aligned}$$

Define $D^*$ and $E$ as

$$\begin{aligned}
D^* &:= \bigsqcup_{n=0}^{N-1} D^*_n \\
E &:= D \backslash D^*
\end{aligned}$$

then

$$\begin{aligned}
\mu_L(D^*)
&= \mu_L\left(
    \bigsqcup_{n=0}^{N-1} D^*_n
\right) \\
&= \sum_{n=0}^{N-1} \mu_L \left(
    D^*_n
\right) \\
&\geq \sum_{n=0}^{N-1} \left(
    \mu_L \left(
        D_n
    \right) - (N+1)\epsilon'
\right) \\
&= \mu_L\left(
    \bigsqcup_{n=1}^{N-1} D_n
\right) - N(N+1)\epsilon' \\
&= \mu_L(D^b) - N(N+1)\epsilon' \\
&= \mu_L(D) - \epsilon - N(N+1)\epsilon'.
\end{aligned}$$

For $x\in D^*$ there exists $n\in [0, 1, \cdots, N]$ such that $x\in D^*_n$, therefore

$$\begin{aligned}
|f(x) - s(x)|
&= |f(x) - s_n(x)| \\
&= \left|
    f(x) - n\frac{M}{N}
\right| \\
&\leq \frac{M}{N} \\
&< \epsilon.
\end{aligned}$$

Thus we proved.

Second, consider the case $f$ is not necessarily non-negative.

Since 

$$\begin{aligned}
f= f^+ - f^-
\end{aligned}$$

for arbitrary $\epsilon>0$ there exists a right-continuous function $s^+$ on $D$ and $E^+\in\mathfrak{M}_L$ with $\mu_L(E^+)<\epsilon$ such that

$$\begin{aligned}
|f^+(x) -s^+(x)| <\epsilon \ \ on \ D \backslash E^+.
\end{aligned}$$

same as $f^-$.

Let $E:=E^+ \cup E^-$ and $s:= s^+ - s^-$, then

$$\begin{aligned}
\mu_L(E)\leq \mu_L(E^+) + \mu_L(E^-)<2\epsilon
\end{aligned}$$

and

$$\begin{aligned}
|f(x) - s(x)|
&= |f^+(x) - f^-(x) - s^+(x) + s^-(x)| \\
&\leq |f^+(x) - s^+(x)| + |f^+(x) -s^-(x)| \\
&< 2\epsilon.
\end{aligned}$$

Thus we proved.

`2.`

Skip.