```
Theorem 1.26
```

Let $\mu$ be a measure on a $\sigma$-algebra $\mathfrak{A}$ of subsetes of a set $X$ and let $(E_n: n \in \mathbb{N})$ be a monotone sequence in $\mathfrak{A}.$

`1.`

If $E_n \uparrow$, then
$$
\lim_{n\rightarrow \infty} \mu (E_n)
=
\mu (\lim_{n\rightarrow \infty} E_n)
$$

`2`.

If $E_n \downarrow$, then
$$
\lim_{n\rightarrow \infty} \mu (E_n)
=
\mu (\lim_{n\rightarrow \infty} E_n),
$$

provided that there exists a set $X \in \mathfrak{A}$ with $\mu(A)<\infty$ such that $E_1\subset A.$


```
proof
```

`1.`

First,
consider there exists $n_0$ such that

$$
\mu(E_{n_0})=\infty.
$$

By the increasing monotonicity of

$$
\{ \ \mu(E_n): n \in \mathbb{N} \ \},
$$

we have

$$
\lim_{n\rightarrow \infty}
\mu(E_n)=\infty.
$$

Also by the increasing monotonicity of

$$
\{
    \ E_n: n\in \mathbb{N} \   
\},
$$

we have

$$
E_{n_0}
\subset
\bigcup_{n \in \mathbb{N}}
E_n,
$$

and by the monotonicity of $\mu$, we have


$$
\begin{aligned}
\infty
&= \mu(E_{n_0}) \\
&\leq
\mu( 
    \bigcup_{n \in \mathbb{N}} E_n
).
\end{aligned}
$$

Thus

$$
\lim_{n\rightarrow \infty} \mu (E_n)
=
\mu (\lim_{n\rightarrow \infty} E_n).
$$

Second, consider the case for any $n\in\mathbb{N}$

$$
\mu(
    E_n
)
<
\infty.
$$

We define

$$
\{ \ 
    F_n: n \in \mathbb{N}
\ \}
$$

such that

$$
F_n
:=
E_n \backslash E_{n-1},
$$

then

$$
\bigcup_{n\in \mathbb{N}}
F_n
=
\bigcup_{n\in \mathbb{N}}
E_n
$$

and for any $n\in \mathbb{N}$

$$
E_n \cap E_{n+1}
=
\emptyset.
$$

So

$$
\begin{aligned}
\mu(
    \bigcup_{n \in \mathbb{N}}
    E_n
)
&=
\mu(
    \bigcup_{n \in \mathbb{N}}
    F_n
) \\
&=
\sum_{n \in \mathbb{N}}
\mu(
    F_n
) \\
&=
\sum_{n \in \mathbb{N}}
\mu(
    E_n \backslash E_{n-1} 
)
\cdots \ 
(\ast)
\end{aligned}
$$

Since

$$
\mu(E_n)
<
\infty,
$$

then

$$
\begin{aligned}
(\ast)
&=
\sum_{n \in \mathbb{N}}
\mu(E_n)
-
\mu(E_{n-1}) \\
&=
\lim_{n\rightarrow \infty}
\mu(E_n)
-
\mu(E_0) \\
&=
\lim_{n\rightarrow \infty}
\mu(E_n)
\end{aligned}
$$

Thus we proved.

`2.`

We define

$$
F_n
:=
E_n \backslash E_{n-1},
$$

then

$$
\bigcap_{n \in \mathbb{N}}
E_n
=
E_1
\backslash
(
    \bigcup_{n \in \mathbb{N}}
    F_n
).
$$

Using this result, we show by the same way of `.1`