```
Theorem 1.14
```

Let f be a mapping of a set X into a set Y. 

Then for an arbitrary collection $\mathfrak{C}$ of subsets of Y, we have 

$$
\sigma \big(f^{-1}(\mathfrak{C}) \big)
=
f^{-1}\big(\sigma(\mathfrak{C})\big)
$$

```
proof
```

First, we can easily show $\subset$ from the fact that the right side is $\sigma$ - algebra and includes $\mathfrak{C}$.

Second, we show $\supset$.

From the fact that $\mathfrak{D}$ below is a $\sigma$ - algebra, 

$$
\mathfrak{D}
:=
\{ A \subset Y: f^{-1}(A) \in \sigma \big( f^{-1}(\mathfrak{C}) \big) \}
$$

and $\mathfrak{D}$ includes $\mathfrak{C}$, this leads to $\mathfrak{D} \supset \sigma(\mathfrak{C})$, and
$f^{-1}(\mathfrak{D}) \supset
f^{-1}\big(\sigma(\mathfrak{C})\big)$.

Also by the definition of $\mathfrak{D}$ it is true that

$$
\sigma \big( f^{-1}(\mathfrak{C}) \big)
\supset
f^{-1}(\mathfrak{D}),
$$

this shows $\supset$.





